Rename eq_term_upto_univ to eq_term_upto

checker/theories/Typing.v
@@ -446,97 +446,97 @@ Inductive red Σ Γ M : term -> Type :=
 Definition R_universe_instance R :=
   fun u u' => Forall2 R (List.map Universe.make u) (List.map Universe.make u').
 
-Inductive eq_term_upto_univ (Re Rle : universe -> universe -> Prop) : term -> term -> Type :=
+Inductive eq_term_upto (Re Rle : universe -> universe -> Prop) : term -> term -> Type :=
 | eq_Rel n  :
-    eq_term_upto_univ Re Rle (tRel n) (tRel n)
+    eq_term_upto Re Rle (tRel n) (tRel n)
 
 | eq_Evar e args args' :
-    All2 (eq_term_upto_univ Re Re) args args' ->
-    eq_term_upto_univ Re Rle (tEvar e args) (tEvar e args')
+    All2 (eq_term_upto Re Re) args args' ->
+    eq_term_upto Re Rle (tEvar e args) (tEvar e args')
 
 | eq_Var id :
-    eq_term_upto_univ Re Rle (tVar id) (tVar id)
+    eq_term_upto Re Rle (tVar id) (tVar id)
 
 | eq_Sort s s' :
     Rle s s' ->
-    eq_term_upto_univ Re Rle (tSort s) (tSort s')
+    eq_term_upto Re Rle (tSort s) (tSort s')
 
 | eq_Cast f f' k T T' :
-    eq_term_upto_univ Re Re f f' ->
-    eq_term_upto_univ Re Re T T' ->
-    eq_term_upto_univ Re Rle (tCast f k T) (tCast f' k T')
+    eq_term_upto Re Re f f' ->
+    eq_term_upto Re Re T T' ->
+    eq_term_upto Re Rle (tCast f k T) (tCast f' k T')
 
 | eq_App t t' args args' :
-    eq_term_upto_univ Re Rle t t' ->
-    All2 (eq_term_upto_univ Re Re) args args' ->
-    eq_term_upto_univ Re Rle (tApp t args) (tApp t' args')
+    eq_term_upto Re Rle t t' ->
+    All2 (eq_term_upto Re Re) args args' ->
+    eq_term_upto Re Rle (tApp t args) (tApp t' args')
 
 | eq_Const c u u' :
     R_universe_instance Re u u' ->
-    eq_term_upto_univ Re Rle (tConst c u) (tConst c u')
+    eq_term_upto Re Rle (tConst c u) (tConst c u')
 
 | eq_Ind i u u' :
     R_universe_instance Re u u' ->
-    eq_term_upto_univ Re Rle (tInd i u) (tInd i u')
+    eq_term_upto Re Rle (tInd i u) (tInd i u')
 
 | eq_Construct i k u u' :
     R_universe_instance Re u u' ->
-    eq_term_upto_univ Re Rle (tConstruct i k u) (tConstruct i k u')
+    eq_term_upto Re Rle (tConstruct i k u) (tConstruct i k u')
 
 | eq_Lambda na na' ty ty' t t' :
-    eq_term_upto_univ Re Re ty ty' ->
-    eq_term_upto_univ Re Rle t t' ->
-    eq_term_upto_univ Re Rle (tLambda na ty t) (tLambda na' ty' t')
+    eq_term_upto Re Re ty ty' ->
+    eq_term_upto Re Rle t t' ->
+    eq_term_upto Re Rle (tLambda na ty t) (tLambda na' ty' t')
 
 | eq_Prod na na' a a' b b' :
-    eq_term_upto_univ Re Re a a' ->
-    eq_term_upto_univ Re Rle b b' ->
-    eq_term_upto_univ Re Rle (tProd na a b) (tProd na' a' b')
+    eq_term_upto Re Re a a' ->
+    eq_term_upto Re Rle b b' ->
+    eq_term_upto Re Rle (tProd na a b) (tProd na' a' b')
 
 | eq_LetIn na na' ty ty' t t' u u' :
-    eq_term_upto_univ Re Re ty ty' ->
-    eq_term_upto_univ Re Re t t' ->
-    eq_term_upto_univ Re Rle u u' ->
-    eq_term_upto_univ Re Rle (tLetIn na ty t u) (tLetIn na' ty' t' u')
+    eq_term_upto Re Re ty ty' ->
+    eq_term_upto Re Re t t' ->
+    eq_term_upto Re Rle u u' ->
+    eq_term_upto Re Rle (tLetIn na ty t u) (tLetIn na' ty' t' u')
 
 | eq_Case ind par p p' c c' brs brs' :
-    eq_term_upto_univ Re Re p p' ->
-    eq_term_upto_univ Re Re c c' ->
+    eq_term_upto Re Re p p' ->
+    eq_term_upto Re Re c c' ->
     All2 (fun x y =>
       fst x = fst y ×
-      eq_term_upto_univ Re Re (snd x) (snd y)
+      eq_term_upto Re Re (snd x) (snd y)
     ) brs brs' ->
-    eq_term_upto_univ Re Rle (tCase (ind, par) p c brs) (tCase (ind, par) p' c' brs')
+    eq_term_upto Re Rle (tCase (ind, par) p c brs) (tCase (ind, par) p' c' brs')
 
 | eq_Proj p c c' :
-    eq_term_upto_univ Re Re c c' ->
-    eq_term_upto_univ Re Rle (tProj p c) (tProj p c')
+    eq_term_upto Re Re c c' ->
+    eq_term_upto Re Rle (tProj p c) (tProj p c')
 
 | eq_Fix mfix mfix' idx :
     All2 (fun x y =>
-      eq_term_upto_univ Re Re x.(dtype) y.(dtype) ×
-      eq_term_upto_univ Re Re x.(dbody) y.(dbody) ×
+      eq_term_upto Re Re x.(dtype) y.(dtype) ×
+      eq_term_upto Re Re x.(dbody) y.(dbody) ×
       x.(rarg) = y.(rarg)
     ) mfix mfix' ->
-    eq_term_upto_univ Re Rle (tFix mfix idx) (tFix mfix' idx)
+    eq_term_upto Re Rle (tFix mfix idx) (tFix mfix' idx)
 
 | eq_CoFix mfix mfix' idx :
     All2 (fun x y =>
-      eq_term_upto_univ Re Re x.(dtype) y.(dtype) ×
-      eq_term_upto_univ Re Re x.(dbody) y.(dbody) ×
+      eq_term_upto Re Re x.(dtype) y.(dtype) ×
+      eq_term_upto Re Re x.(dbody) y.(dbody) ×
       x.(rarg) = y.(rarg)
     ) mfix mfix' ->
-    eq_term_upto_univ Re Rle (tCoFix mfix idx) (tCoFix mfix' idx).
+    eq_term_upto Re Rle (tCoFix mfix idx) (tCoFix mfix' idx).
 
 Definition eq_term `{checker_flags} φ :=
-  eq_term_upto_univ (eq_universe φ) (eq_universe φ).
+  eq_term_upto (eq_universe φ) (eq_universe φ).
 
 (* ** Syntactic cumulativity up-to universes
 
   We shouldn't look at printing annotations *)
 
 Definition leq_term `{checker_flags} φ :=
-  eq_term_upto_univ (eq_universe φ) (leq_universe φ).
+  eq_term_upto (eq_universe φ) (leq_universe φ).
 
 Fixpoint strip_casts t :=
   match t with
